

# Laurent Series Expansion of $f(z) = \frac{1}{(z^2+1)(z-2)}$ in the Annulus $1 < |z| < 2$

## Summary

- **a. Verdict:** The Laurent series expansion in the annulus  $1 < |z| < 2$  has been successfully computed.
- **b. Method Sketch:**

1. Perform partial fraction decomposition over the real numbers:

$$f(z) = \frac{Az + B}{z^2 + 1} + \frac{C}{z - 2}$$

Solving yields  $A = -1/5$ ,  $B = -2/5$ , and  $C = 1/5$ .

2. For  $|z| > 1$ , expand the term containing  $z^2 + 1$  in powers of  $1/z$  using the geometric series with  $w = -1/z^2$ .
3. For  $|z| < 2$ , expand the term containing  $z-2$  in powers of  $z$  using the geometric series with ratio  $z/2$ .
4. Combine the two series to obtain the complete Laurent series valid in the annulus  $1 < |z| < 2$ .

## Detailed Solution

### Step 1: Partial Fraction Decomposition

We perform partial fraction decomposition of  $f(z)$  in the form:

$$f(z) = \frac{1}{(z^2 + 1)(z - 2)} = \frac{Az + B}{z^2 + 1} + \frac{C}{z - 2}.$$

Multiplying both sides by the common denominator  $(z^2 + 1)(z - 2)$  gives:

$$1 = (Az + B)(z - 2) + C(z^2 + 1).$$

To determine  $C$ , evaluate at  $z = 2$ :

$$1 = (2A + B)(0) + C(2^2 + 1) \implies 1 = 5C \implies C = \frac{1}{5}.$$

To find  $A$  and  $B$ , expand the right-hand side and collect powers of  $z$ :

$$1 = (Az^2 - 2Az + Bz - 2B) + C(z^2 + 1) = (A + C)z^2 + (-2A + B)z + (-2B + C).$$

Comparing coefficients:

$$\begin{aligned} A + C &= 0 \implies A = -C = -\frac{1}{5}, \\ -2A + B &= 0 \implies B = 2A = -\frac{2}{5}. \end{aligned}$$

Thus, the decomposition is:

$$f(z) = -\frac{1}{5} \cdot \frac{z+2}{z^2+1} + \frac{1}{5} \cdot \frac{1}{z-2}.$$

## Step 2: Expansion in the Annulus $1 < |z| < 2$

We expand each term into a series convergent in the given annulus.

### Part A: Expansion of $-\frac{1}{5} \frac{z+2}{z^2+1}$

This term has singularities at  $z = \pm i$ . Since  $|z| > 1$  in the annulus, we have  $|z^2| > 1$ , i.e.,  $|-1/z^2| < 1$ . We rewrite:

$$\frac{z+2}{z^2+1} = \frac{z+2}{z^2(1+z^{-2})} = (z^{-1} + 2z^{-2}) \cdot \frac{1}{1 - (-z^{-2})}.$$

Using the geometric series  $\frac{1}{1-w} = \sum_{k=0}^{\infty} w^k$  with  $w = -z^{-2}$ :

$$\frac{z+2}{z^2+1} = (z^{-1} + 2z^{-2}) \sum_{k=0}^{\infty} (-1)^k z^{-2k}.$$

Distributing the sums:

$$\frac{z+2}{z^2+1} = \sum_{k=0}^{\infty} (-1)^k z^{-2k-1} + \sum_{k=0}^{\infty} 2(-1)^k z^{-2k-2}.$$

Multiplying by  $-\frac{1}{5}$ :

$$-\frac{1}{5} \frac{z+2}{z^2+1} = \sum_{k=0}^{\infty} \frac{(-1)^{k+1}}{5} z^{-(2k+1)} + \sum_{k=0}^{\infty} \frac{2(-1)^{k+1}}{5} z^{-(2k+2)}.$$

This gives the principal part of the Laurent series.

### Part B: Expansion of $\frac{1}{5} \frac{1}{z-2}$

This term has a singularity at  $z = 2$ . Since  $|z| < 2$  in the annulus, we have  $|z/2| < 1$ . We rewrite:

$$\frac{1}{z-2} = \frac{1}{-2(1-z/2)} = -\frac{1}{2} \sum_{n=0}^{\infty} \left(\frac{z}{2}\right)^n = -\sum_{n=0}^{\infty} \frac{z^n}{2^{n+1}}.$$

Multiplying by  $\frac{1}{5}$ :

$$\frac{1}{5} \frac{1}{z-2} = -\sum_{n=0}^{\infty} \frac{1}{5 \cdot 2^{n+1}} z^n.$$

This gives the analytic part of the Laurent series.

### Step 3: Final Laurent Series

Combining both parts, the Laurent series for  $f(z)$  in the annulus  $1 < |z| < 2$  is:

$$f(z) = \sum_{k=0}^{\infty} \frac{(-1)^{k+1}}{5} z^{-(2k+1)} + \sum_{k=0}^{\infty} \frac{2(-1)^{k+1}}{5} z^{-(2k+2)} - \sum_{n=0}^{\infty} \frac{1}{5 \cdot 2^{n+1}} z^n.$$

Writing the first few terms explicitly:

$$f(z) = \cdots + \frac{2}{5}z^{-4} + \frac{1}{5}z^{-3} - \frac{2}{5}z^{-2} - \frac{1}{5}z^{-1} - \frac{1}{10} - \frac{1}{20}z - \frac{1}{40}z^2 - \cdots$$